Check genesis RLP in run_test
Progress on #69

tests/vfmTestHelperScript.sml
@@ -11,28 +11,112 @@ Datatype:
   test_result
   = Passed
   | GenesisBlockDecodeFailure
+  | GenesisBlockDecodeMismatch
   | GenesisHeaderMismatch bytes32
   | GenesisStateMismatch bytes32
   | ExpectedException string
   | ExceptionMismatch
   | UnexpectedException
   | BlockDecodeFailure
+  | BlockDecodeMismatch
   | LastHashMismatch bytes32
   | StateMismatch
   | OutOfFuel
 End
 
+(* TODO: move to another theory? *)
+
+Definition block_header_from_block_rlp_def:
+  block_header_from_block_rlp rlp =
+  if ¬is_RLPL rlp then NONE else
+  let ls = dest_RLPL rlp in
+  if LENGTH ls ≠ 4 then NONE else
+  let rlp = EL 0 ls in
+  if ¬is_RLPL rlp then NONE else
+  let ls = dest_RLPL rlp in
+  if ¬(LENGTH ls = 20 ∧ EVERY is_RLPB ls) then NONE else
+  let coinbase   = dest_RLPB (EL  2 ls) in
+  let stateRoot  = dest_RLPB (EL  3 ls) in
+  let number     = dest_RLPB (EL  8 ls) in
+  let gasLimit   = dest_RLPB (EL  9 ls) in
+  let gasUsed    = dest_RLPB (EL 10 ls) in
+  let timestamp  = dest_RLPB (EL 11 ls) in
+  let prevRandao = dest_RLPB (EL 13 ls) in
+  let baseFeePerGas = dest_RLPB (EL 15 ls) in
+  let blobGasUsed   = dest_RLPB (EL 17 ls) in
+  let excessBlobGas = dest_RLPB (EL 18 ls) in
+  let parentBeaconBlockRoot = dest_RLPB (EL 19 ls) in
+  (*
+     parentHash;
+     ommersHash;
+     coinbase;
+     stateRoot;
+     transactionsRoot;
+     receiptRoot;
+     bloom;
+     difficulty;
+     number;
+     gasLimit;
+     gasUsed;
+     timestamp;
+     extraData;
+     prevRandao;
+     nonce;
+     baseFeePerGas;
+     withdrawalsRoot;
+     blobGasUsed;
+     excessBlobGas;
+     parentBeaconBlockRoot
+   *)
+    SOME
+    <| baseFeePerGas := num_of_be_bytes baseFeePerGas
+     ; excessBlobGas := num_of_be_bytes excessBlobGas
+     ; gasUsed       := num_of_be_bytes gasUsed
+     ; blobGasUsed   := num_of_be_bytes blobGasUsed
+     ; number        := num_of_be_bytes number
+     ; timeStamp     := num_of_be_bytes timestamp
+     ; coinBase      := word_of_bytes T 0w coinbase
+     ; gasLimit      := num_of_be_bytes gasLimit
+     ; prevRandao    := word_of_bytes T 0w prevRandao
+     ; parentBeaconBlockRoot := word_of_bytes T 0w parentBeaconBlockRoot
+     ; stateRoot     := word_of_bytes T 0w stateRoot
+     (* not in header *)
+     ; hash          := 0w
+     ; transactions  := []
+     ; withdrawals   := []
+     |>
+End
+
+val block_header_from_block_rlp_pre_def =
+  cv_auto_trans_pre block_header_from_block_rlp_def;
+
+Theorem block_header_from_block_rlp_pre[cv_pre]:
+  block_header_from_block_rlp_pre x
+Proof
+  rw[block_header_from_block_rlp_pre_def]
+  \\ Cases_on`x` \\ gvs[]
+  \\ strip_tac \\ gvs[]
+QED
+
 Definition run_test_def:
   run_test fuel
     preState
-    (genesisRLP: byte list) (* TODO: check RLP decoding *)
+    (genesisRLP: byte list)
     (genesisBlock: block)
     validBlocks
     lastBlockHash
     postState
     expectException
   =
-    case state_root_clocked fuel preState
+    case rlp_decode genesisRLP
+    of NONE => GenesisBlockDecodeFailure |
+    SOME rlp =>
+    case block_header_from_block_rlp rlp
+    of NONE => GenesisBlockDecodeFailure |
+    SOME genesisHeader =>
+    if genesisHeader with hash := genesisBlock.hash <> genesisBlock
+    then GenesisBlockDecodeMismatch
+    else case state_root_clocked fuel preState
     of NONE => OutOfFuel |
     SOME preStateRootBytes =>
     let preStateRoot = word_of_bytes T 0w preStateRootBytes in
